Unification and contract establishment

hol/symb_exec/p4_symb_exec_test1Script.sml
@@ -6,6 +6,11 @@ open p4_symb_execLib;
 
 val _ = new_theory "p4_symb_exec_test1";
 
+(* Test 1:
+ * There's a single if-statement that branches on symbolic bits.
+ * Postcondition holds regardless of which path was taken.
+ *
+ * This tests if basic branching and unification works. *)
 
 val symb_exec1_actx = ``([arch_block_inp;
   arch_block_pbl "p"
@@ -107,6 +112,8 @@ val symb_exec1_actx = ``([arch_block_inp;
     ("write",[("this",d_in); ("index",d_in); ("value",d_in)],register_write)])],
  [("NoAction",stmt_seq stmt_empty (stmt_ret (e_v v_bot)),[])]):v1model_ascope actx``;
 
+(*
+(* Concrete state from old example program *)
 val symb_exec1_astate = rhs $ concl $ EVAL “(p4_append_input_list [([F; F; F; F; F; F; F; T; F; F; F; T; F; F; F; T; F; F; F; T; F; F; F; T; F;
    F; F; F; F; F; F; F; F; F; F; F; F; F; F; F; T; F; T; T; F; F; F; F],0);
  ([F; F; F; F; F; F; T; F; F; F; F; T; F; F; F; T; T; F; F; F; F; F; F; T; F;
@@ -115,16 +122,22 @@ val symb_exec1_astate = rhs $ concl $ EVAL “(p4_append_input_list [([F; F; F; 
    F; F; F; F; F; F; F; F; F; F; F; F; F; F; F; T; F; T; T; F; F; F; F],0);
  ([T; T; T; T; F; T; F; F; F; F; F; T; F; F; F; T; F; F; F; T; F; F; F; T; F;
    F; F; F; F; F; F; F; F; F; F; F; F; F; F; F; T; F; T; T; F; F; F; F],0)] (((0,[],[],ARB,ARB,ARB,[]),[[]],arch_frame_list_empty,status_running):v1model_ascope astate))”;
-
+*)
 
 (*
 (* eval_under_assum: *)
 GEN_ALL $ eval_under_assum p4_v1modelLib.v1model_arch_ty symb_exec1_actx symb_exec1_astate [] [] (ASSUME T) 10;
 *)
 
+(* As symbolic packet, generate something like this:
+  
+   data = [b1; b2; b3; b4; b5; b6; b7; b8]
+   port = p
+
+*)
+
 val symb_exec1_astate_symb = rhs $ concl $ EVAL “(p4_append_input_list [([e1; e2; e3; e4; e5; e6; e7; e8; F; F; F; T; F; F; F; T; F; F; F; T; F; F; F; T; F;
    F; F; F; F; F; F; F; F; F; F; F; F; F; F; F; T; F; T; T; F; F; F; F],0)] (((0,[],[],ARB,ARB,ARB,[]),[[]],arch_frame_list_empty,status_running):v1model_ascope astate))”;
-
 
 
 (* symb_exec: *)
@@ -136,25 +149,98 @@ val stop_consts_rewr = []
 val stop_consts_never = []
 val path_cond = (ASSUME T)
 val fuel = 2
-(*
+(* For debugging:
 val comp_thm = INST_TYPE [Type.alpha |-> arch_ty] arch_multi_exec_comp_n_tl_assl
 *)
 
-(* Before branch
-val [(path_cond, step_thm)] =
- symb_exec arch_ty ctx init_astate stop_consts_rewr stop_consts_never path_cond 24
+(* For debugging, branch happens here:
+val [(path_cond_res, step_thm), (path_cond2_res, step_thm2)] =
+ symb_exec arch_ty ctx init_astate stop_consts_rewr stop_consts_never path_cond 25;
 *)
 
-(* Branch happens here *)
-val [(path_cond, step_thm), (path_cond2, step_thm2)] =
- symb_exec arch_ty ctx init_astate stop_consts_rewr stop_consts_never path_cond 25
+(* Finishes at 45 steps (one step of which is a symbolic branch)
+ * (higher numbers as arguments will work, but do no extra computations) *)
 
+val [(path_cond_res, step_thm), (path_cond2_res, step_thm2)] =
+ symb_exec arch_ty ctx init_astate stop_consts_rewr stop_consts_never path_cond 50;
+
+open p4_auxTheory;
+
+(*******************************)
+(* Step 1: prove postcondition *)
+
+(* True if the output packet queue contains a single packet with
+ * the provided output port *)
+Definition packet_has_port_def:
+ packet_has_port (((i, in_out_list, in_out_list', scope), g_scope_list, arch_frame_list, status):'a astate) port_ok =
+  case in_out_list' of
+    [] => F
+  | [(data, port)] => port = port_ok
+  | _ => F
+End
+
+val postcond = “(\s. packet_has_port s 1 \/ packet_has_port s 2):v1model_ascope astate -> bool”;
+
+Theorem symb_exec_add_postcond:
+!P f s s' Q.
+(P ==> f s = SOME s') ==>
+Q s' ==>
+(P ==> f s = SOME s' /\ Q s')
+Proof
+metis_tac []
+QED
+
+val step_thm' = HO_MATCH_MP symb_exec_add_postcond step_thm;
+val postcond_thm = EQT_ELIM $ SIMP_CONV (srw_ss()) [packet_has_port_def] $ mk_comb (postcond, the_final_state_imp step_thm);
+val step_postcond_thm = MATCH_MP step_thm' postcond_thm;
+
+val step_thm2' = HO_MATCH_MP symb_exec_add_postcond step_thm2;
+val postcond_thm2 = EQT_ELIM $ SIMP_CONV (srw_ss()) [packet_has_port_def] $ mk_comb (postcond, the_final_state_imp step_thm2);
+val step_postcond_thm2 = MATCH_MP step_thm2' postcond_thm2;
+
+(**************************************)
+(* Step 2: rewrite into contract form *)
+
+(* TODO: Eliminate n, put initial state in precondition somehow? *)
+Definition p4_contract_def:
+ p4_contract P ctx s n Q =
+  (P ==> arch_multi_exec ctx s n <> NONE /\ !s'. arch_multi_exec ctx s n = SOME s' ==> Q s')
+End
+
+Theorem p4_exec_univ:
+!P ctx s n s' Q.
+(P ==> arch_multi_exec ctx s n = SOME s' /\ Q s') ==>
+p4_contract P ctx s n Q
 (*
-val [(path_cond, step_thm), (path_cond2, step_thm2)] =
- symb_exec arch_ty ctx init_astate stop_consts_rewr stop_consts_never path_cond 26
-
-val [(path_cond, step_thm), (path_cond2, step_thm2)] =
- symb_exec arch_ty ctx init_astate stop_consts_rewr stop_consts_never path_cond 28
+(P ==> arch_multi_exec ctx s n <> NONE /\ !s'. arch_multi_exec ctx s n = SOME s' ==> Q s')
 *)
+Proof
+fs[p4_contract_def]
+QED
+
+val step_postcond_ct_thm = MATCH_MP p4_exec_univ step_postcond_thm
+val step_postcond_ct_thm2 = MATCH_MP p4_exec_univ step_postcond_thm2
+
+(***********************)
+(* Step 3: unification *)
+
+Theorem p4_symb_exec_unify:
+(*
+!P1 P2 f s Q.
+(P1 /\ P2 ==> f s <> NONE /\ !s'. f s = SOME s' ==> Q s') ==>
+(~P1 /\ P2 ==> f s <> NONE /\ !s'. f s = SOME s' ==> Q s') ==>
+P2 ==> f s <> NONE /\ !s'. f s = SOME s' ==> Q s'
+*)
+!P1 P2 ctx s n Q.
+p4_contract (P1 /\ P2) ctx s n Q ==>
+p4_contract (~P1 /\ P2) ctx s n Q ==>
+p4_contract P2 ctx s n Q
+Proof
+fs[p4_contract_def] >>
+metis_tac []
+QED
+
+val thm1 = MATCH_MP p4_symb_exec_unify step_postcond_ct_thm
+val thm2 = MATCH_MP thm1 step_postcond_ct_thm2
 
 val _ = export_theory ();
